ok
git-svn-id: svn://scm.gforge.inria.fr/svn/cfml@92 ba02c806-7d2b-4818-9a48-35b22e6bdc79

demo/test.ml
@@ -4,7 +4,7 @@
 let p = 
    let x = ref 3 in
    let y = !x in
-   x := 4
+   x := 4;
    let z = !x in
    y + z
 
